tweak definition of flatten to use an index rather than check the length of the output accumulator--this prevents the accumulator from repeatedly showing up in the expression and making the term huge

src/Experiments/SimplyTypedArithmetic.v
@@ -1245,12 +1245,17 @@ Module Rows.
       Local Notation fw := (fun i => weight (S i) / weight i) (only parsing).
 
       Section SumRows.
-        Definition sum_rows' start_state (row1 row2 : list Z) : list Z * Z :=
-          fold_right (fun next (state : list Z * Z) =>
-                        let i := length (fst state) in (* length of output accumulator tells us the index of [next] *)
-                          dlet_nd sum_carry := Z.add_with_get_carry_full (fw i) (snd state) (fst next) (snd next) in
-                          (fst state ++ [fst sum_carry], snd sum_carry)) start_state (rev (combine row1 row2)).
-        Definition sum_rows := sum_rows' (nil,0).
+        Definition sum_rows' start_state (row1 row2 : list Z) : list Z * Z * nat :=
+          fold_right (fun next (state : list Z * Z * nat) =>
+                        let i := snd state in
+                        let low_high' :=
+                            dlet_nd low_high := fst state in
+                            let low := fst low_high in
+                            let high := snd low_high in
+                          dlet_nd sum_carry := Z.add_with_get_carry_full (fw i) high (fst next) (snd next) in
+                          (low ++ [fst sum_carry], snd sum_carry) in
+                     (low_high', S i)) start_state (rev (combine row1 row2)).
+        Definition sum_rows row1 row2 := fst (sum_rows' (nil, 0, 0%nat) row1 row2).
 
         Ltac push :=
           repeat match goal with
@@ -1273,7 +1278,9 @@ Module Rows.
 
         Lemma sum_rows'_cons state x1 row1 x2 row2 :
           sum_rows' state (x1 :: row1) (x2 :: row2) =
-          sum_rows' (fst state ++ [(snd state + x1 + x2) mod (fw (length (fst state)))], (snd state + x1 + x2) / fw (length (fst state))) row1 row2.
+          sum_rows' (fst (fst state) ++ [(snd (fst state) + x1 + x2) mod (fw (snd state))],
+                     (snd (fst state) + x1 + x2) / fw (snd state),
+                     S (snd state)) row1 row2.
         Proof.
           cbv [sum_rows' Let_In]; autorewrite with push_combine.
           rewrite !fold_left_rev_right. cbn [fold_left].
@@ -1288,20 +1295,21 @@ Module Rows.
 
         Lemma sum_rows'_div_mod_length row1 :
           forall nm start_state row2 row1' row2',
-            let m := length (fst start_state) in
+            let m := snd start_state in
             let n := length row1 in
             length row2 = n ->
             length row1' = m ->
             length row2' = m ->
+            length (fst (fst start_state)) = m ->
             (nm = n + m)%nat ->
             let eval := Positional.eval weight in
-            is_div_mod (eval m) start_state (eval m row1' + eval m row2') (weight m) ->
-            length (fst (sum_rows' start_state row1 row2)) = nm
-            /\ is_div_mod (eval nm) (sum_rows' start_state row1 row2)
+            is_div_mod (eval m) (fst start_state) (eval m row1' + eval m row2') (weight m) ->
+            length (fst (fst (sum_rows' start_state row1 row2))) = nm
+            /\ is_div_mod (eval nm) (fst (sum_rows' start_state row1 row2))
                           (eval nm (row1' ++ row1) + eval nm (row2' ++ row2))
                           (weight nm).
         Proof.
-          induction row1 as [|x1 row1]; destruct row2 as [|x2 row2]; intros; subst nm; push; [].
+          induction row1 as [|x1 row1]; destruct row2 as [|x2 row2]; intros; subst nm; push; [ ].
           rewrite (app_cons_app_app _ row1'), (app_cons_app_app _ row2').
           apply IHrow1; clear IHrow1; autorewrite with cancel_pair distr_length in *; try omega.
           eapply is_div_mod_step with (x := x1 + x2); try eassumption; push.
@@ -1330,18 +1338,19 @@ Module Rows.
 
         Lemma sum_rows'_partitions row1 :
           forall nm start_state row2 row1' row2',
-            let m := length (fst start_state) in
+            let m := snd start_state in
             let n := length row1 in
             length row2 = n ->
             length row1' = m ->
             length row2' = m ->
+            length (fst (fst start_state)) = m ->
             nm = (n + m)%nat ->
             let eval := Positional.eval weight in
-            snd start_state = (eval m row1' + eval m row2') / weight m ->
+            snd (fst start_state) = (eval m row1' + eval m row2') / weight m ->
             (forall j, (j < m)%nat ->
-                       nth_default 0 (fst start_state) j = ((eval m row1' + eval m row2') mod (weight (S j))) / (weight j)) ->
+                       nth_default 0 (fst (fst start_state)) j = ((eval m row1' + eval m row2') mod (weight (S j))) / (weight j)) ->
             forall i, (i < nm)%nat ->
-                      nth_default 0 (fst (sum_rows' start_state row1 row2)) i
+                      nth_default 0 (fst (fst (sum_rows' start_state row1 row2))) i
                       = ((eval nm (row1' ++ row1) + eval nm (row2' ++ row2)) mod (weight (S i))) / (weight i).
         Proof.
           induction row1 as [|x1 row1]; destruct row2 as [|x2 row2]; intros; subst nm; push; [].
@@ -1351,14 +1360,14 @@ Module Rows.
             repeat match goal with
                    | H : ?LHS = _ |- _ =>
                      match LHS with context [start_state] => rewrite H end
-                   | H : context [nth_default 0 (fst start_state)] |- _ => rewrite H by omega
+                   | H : context [nth_default 0 (fst (fst start_state))] |- _ => rewrite H by omega
                    | _ => rewrite <-(Z.add_assoc _ x1 x2)
                    end.
           { rewrite div_step by auto using Z.gt_lt.
             rewrite Z.mul_div_eq_full by auto; rewrite weight_multiples by auto. push. }
-          { rewrite weight_div_mod with (j:=length (fst start_state)) (i:=S j) by (auto; omega).
+          { rewrite weight_div_mod with (j:=snd start_state) (i:=S j) by (auto; omega).
             push_Zmod. autorewrite with zsimplify_fast. reflexivity. }
-          { push. replace (length (fst start_state)) with j in * by omega.
+          { push. replace (snd start_state) with j in * by omega.
             push. rewrite add_mod_div_multiple by auto using Z.lt_le_incl.
             push. }
         Qed.
